theory/Sound_Semantics.thy
@@ -817,45 +817,78 @@ qed
 
 theorem may_be_static_eval_state_preserved_under_step : "
   \<lbrakk>
+    (\<V>, \<C>) \<Turnstile>\<^sub>\<sigma> \<langle>LET x = b in e; \<rho>; \<kappa>\<rangle>; 
+    seq_step (b, \<rho>) \<omega>
+  \<rbrakk> \<Longrightarrow>
+  (\<V>, \<C>) \<Turnstile>\<^sub>\<sigma> \<langle>e;\<rho>(x \<mapsto> \<omega>);\<kappa>\<rangle>
+"
+proof -
+  assume 
+    H1: "(\<V>, \<C>) \<Turnstile>\<^sub>\<sigma> \<langle>LET x = b in e; \<rho>; \<kappa>\<rangle>" and
+    H2: "seq_step (b, \<rho>) \<omega>"
+    
+  from H2 show "(\<V>, \<C>) \<Turnstile>\<^sub>\<sigma> \<langle>e;\<rho>(x \<mapsto> \<omega>);\<kappa>\<rangle>"
+  proof cases
+    case Let_Unit
+    
+    assume
+      H3: "b = \<lparr>\<rparr>" and
+      H4: "\<omega> = VUnit"
+
+    from H1 H3 have "(\<V>, \<C>) \<Turnstile>\<^sub>\<sigma> \<langle>LET x = \<lparr>\<rparr> in e; \<rho>; \<kappa>\<rangle>" by simp
+
+    then have "(\<V>, \<C>) \<Turnstile>\<^sub>\<sigma> \<langle>e; \<rho> ++ [x \<mapsto> VUnit]; \<kappa>\<rangle>" by (simp add: may_be_static_eval_state_to_state_let_unit)
+    
+    with H4 show "(\<V>, \<C>) \<Turnstile>\<^sub>\<sigma> \<langle>e;\<rho>(x \<mapsto> \<omega>);\<kappa>\<rangle>" by simp
+  next
+    case (Let_Prim p)
+
+    assume
+      H3: "b = Prim p" and
+      H4: "\<omega> = VClosure p \<rho>"
+
+    from H1 H3 have "(\<V>, \<C>) \<Turnstile>\<^sub>\<sigma> \<langle>LET x = Prim p in e; \<rho>; \<kappa>\<rangle>" by simp
+
+    then have "(\<V>, \<C>) \<Turnstile>\<^sub>\<sigma> \<langle>e; \<rho> ++ [x \<mapsto> VClosure p \<rho>]; \<kappa>\<rangle>" by (simp add: may_be_static_eval_state_to_state_let_prim)
+    
+    with H4 show "(\<V>, \<C>) \<Turnstile>\<^sub>\<sigma> \<langle>e;\<rho>(x \<mapsto> \<omega>);\<kappa>\<rangle>" by simp
+  next
+    case (Let_Fst x\<^sub>p x\<^sub>1 x\<^sub>2 \<rho>\<^sub>p)
+
+    assume 
+      H3: "b = FST x\<^sub>p" and
+      H4: "\<rho> x\<^sub>p = Some (VClosure (prim.Pair x\<^sub>1 x\<^sub>2) \<rho>\<^sub>p)" and
+      H5: "\<rho>\<^sub>p x\<^sub>1 = Some \<omega>"
+
+    from H1 H3 have "(\<V>, \<C>) \<Turnstile>\<^sub>\<sigma> \<langle>LET x = FST x\<^sub>p in e; \<rho>; \<kappa>\<rangle>" by simp
+
+    with H4 H5 show "(\<V>, \<C>) \<Turnstile>\<^sub>\<sigma> \<langle>e; \<rho>(x \<mapsto> \<omega>); \<kappa>\<rangle>" by (simp add: may_be_static_eval_state_to_state_let_fst)
+  next
+    case (Let_Snd x\<^sub>p x\<^sub>1 x\<^sub>2 \<rho>\<^sub>p)
+
+    assume 
+      H3: "b = SND x\<^sub>p" and
+      H4: "\<rho> x\<^sub>p = Some (VClosure (prim.Pair x\<^sub>1 x\<^sub>2) \<rho>\<^sub>p)" and
+      H5: "\<rho>\<^sub>p x\<^sub>2 = Some \<omega>"
+
+    from H1 H3 have "(\<V>, \<C>) \<Turnstile>\<^sub>\<sigma> \<langle>LET x = SND x\<^sub>p in e; \<rho>; \<kappa>\<rangle>" by simp
+
+    with H4 H5 show "(\<V>, \<C>) \<Turnstile>\<^sub>\<sigma> \<langle>e; \<rho>(x \<mapsto> \<omega>); \<kappa>\<rangle>" by (simp add: may_be_static_eval_state_to_state_let_snd)
+  qed
+qed
+
+theorem may_be_static_eval_state_preserved_under_step_up : "
+  \<lbrakk>
     (\<V>, \<C>) \<Turnstile>\<^sub>\<sigma> \<sigma>; 
-    \<sigma> \<hookrightarrow> \<sigma>'
+    \<sigma> \<up>\<hookrightarrow> \<sigma>'
   \<rbrakk> \<Longrightarrow>
   (\<V>, \<C>) \<Turnstile>\<^sub>\<sigma> \<sigma>'
 "
 proof -
   assume "(\<V>, \<C>) \<Turnstile>\<^sub>\<sigma> \<sigma>"
-  assume "\<sigma> \<hookrightarrow> \<sigma>'" then
+  assume "\<sigma> \<up>\<hookrightarrow> \<sigma>'" then
   show "(\<V>, \<C>) \<Turnstile>\<^sub>\<sigma> \<sigma>'"
   proof cases
-    case (Result \<rho> x \<omega> x\<^sub>\<kappa> e\<^sub>\<kappa> \<rho>\<^sub>\<kappa> \<kappa>)
-    assume "\<sigma> = \<langle>RESULT x;\<rho>;\<langle>x\<^sub>\<kappa>,e\<^sub>\<kappa>,\<rho>\<^sub>\<kappa>\<rangle> # \<kappa>\<rangle>" and "\<sigma>' = \<langle>e\<^sub>\<kappa>;\<rho>\<^sub>\<kappa> ++ [x\<^sub>\<kappa> \<mapsto> \<omega>];\<kappa>\<rangle>" and "\<rho> x = Some \<omega>" 
-    with `(\<V>, \<C>) \<Turnstile>\<^sub>\<sigma> \<sigma>`
-    show "(\<V>, \<C>) \<Turnstile>\<^sub>\<sigma> \<sigma>'" by (simp add: may_be_static_eval_state_to_state_result)
-  next
-    case (Let_Unit x e \<rho> \<kappa>)
-    assume "\<sigma> = \<langle>LET x = \<lparr>\<rparr> in e;\<rho>;\<kappa>\<rangle>" and "\<sigma>' = \<langle>e;\<rho> ++ [x \<mapsto> VUnit];\<kappa>\<rangle>"
-    with `(\<V>, \<C>) \<Turnstile>\<^sub>\<sigma> \<sigma>`
-    show "(\<V>, \<C>) \<Turnstile>\<^sub>\<sigma> \<sigma>'" by (simp add: may_be_static_eval_state_to_state_let_unit)
-  next
-    case (Let_Prim x p e \<rho> \<kappa>)
-    assume "\<sigma> = \<langle>LET x = Prim p in e;\<rho>;\<kappa>\<rangle>" and "\<sigma>' = \<langle>e;\<rho> ++ [x \<mapsto> (VClosure p \<rho>)];\<kappa>\<rangle>"
-    with `(\<V>, \<C>) \<Turnstile>\<^sub>\<sigma> \<sigma>`
-    show "(\<V>, \<C>) \<Turnstile>\<^sub>\<sigma> \<sigma>'" by (simp add: may_be_static_eval_state_to_state_let_prim)
-  next
-    case (Let_Fst \<rho> x\<^sub>p x\<^sub>1 x\<^sub>2 \<rho>\<^sub>p \<omega> x e \<kappa>)
-    assume "\<sigma> = \<langle>LET x = FST x\<^sub>p in e;\<rho>;\<kappa>\<rangle>"
-    and "\<sigma>' = \<langle>e;\<rho> ++ [x \<mapsto> \<omega>];\<kappa>\<rangle>"
-    and "\<rho> x\<^sub>p = Some (VClosure (Pair x\<^sub>1 x\<^sub>2) \<rho>\<^sub>p)" and "\<rho>\<^sub>p x\<^sub>1 = Some \<omega>"
-    with `(\<V>, \<C>) \<Turnstile>\<^sub>\<sigma> \<sigma>`
-    show "(\<V>, \<C>) \<Turnstile>\<^sub>\<sigma> \<sigma>'" by (simp add: may_be_static_eval_state_to_state_let_fst)
-  next
-    case (Let_Snd \<rho> x\<^sub>p x\<^sub>1 x\<^sub>2 \<rho>\<^sub>p \<omega> x e \<kappa>)
-    assume "\<sigma> = \<langle>LET x = SND x\<^sub>p in e;\<rho>;\<kappa>\<rangle>"
-    and "\<sigma>' = \<langle>e;\<rho> ++ [x \<mapsto> \<omega>];\<kappa>\<rangle>"
-    and "\<rho> x\<^sub>p = Some (VClosure (Pair x\<^sub>1 x\<^sub>2) \<rho>\<^sub>p)" and "\<rho>\<^sub>p x\<^sub>2 = Some \<omega>"
-    with `(\<V>, \<C>) \<Turnstile>\<^sub>\<sigma> \<sigma>`
-    show "(\<V>, \<C>) \<Turnstile>\<^sub>\<sigma> \<sigma>'" by (simp add: may_be_static_eval_state_to_state_let_snd)
-  next
     case (Let_Case_Left \<rho> x\<^sub>s x\<^sub>l' \<rho>\<^sub>l \<omega>\<^sub>l x x\<^sub>l e\<^sub>l x\<^sub>r e\<^sub>r e \<kappa>)
     assume "\<sigma> = \<langle>LET x = CASE x\<^sub>s LEFT x\<^sub>l |> e\<^sub>l RIGHT x\<^sub>r |> e\<^sub>r in e;\<rho>;\<kappa>\<rangle>"
     and "\<sigma>' = \<langle>e\<^sub>l;\<rho> ++ [x\<^sub>l \<mapsto> \<omega>\<^sub>l];\<langle>x,e,\<rho>\<rangle> # \<kappa>\<rangle>"
@@ -882,17 +915,37 @@ proof -
 
 qed
 
+theorem may_be_static_eval_state_preserved_under_step_down : "
+  \<lbrakk>
+    (\<V>, \<C>) \<Turnstile>\<^sub>\<sigma> \<sigma>; 
+    \<sigma> \<down>\<hookrightarrow> \<sigma>'
+  \<rbrakk> \<Longrightarrow>
+  (\<V>, \<C>) \<Turnstile>\<^sub>\<sigma> \<sigma>'
+"
+proof -
+  assume "(\<V>, \<C>) \<Turnstile>\<^sub>\<sigma> \<sigma>"
+  assume "\<sigma> \<down>\<hookrightarrow> \<sigma>'" then
+  show "(\<V>, \<C>) \<Turnstile>\<^sub>\<sigma> \<sigma>'"
+  proof cases
+    case (Result \<rho> x \<omega> x\<^sub>\<kappa> e\<^sub>\<kappa> \<rho>\<^sub>\<kappa> \<kappa>)
+    assume "\<sigma> = \<langle>RESULT x;\<rho>;\<langle>x\<^sub>\<kappa>,e\<^sub>\<kappa>,\<rho>\<^sub>\<kappa>\<rangle> # \<kappa>\<rangle>" and "\<sigma>' = \<langle>e\<^sub>\<kappa>;\<rho>\<^sub>\<kappa> ++ [x\<^sub>\<kappa> \<mapsto> \<omega>];\<kappa>\<rangle>" and "\<rho> x = Some \<omega>" 
+    with `(\<V>, \<C>) \<Turnstile>\<^sub>\<sigma> \<sigma>`
+    show "(\<V>, \<C>) \<Turnstile>\<^sub>\<sigma> \<sigma>'" by (simp add: may_be_static_eval_state_to_state_result)
+  qed
+
+qed
+
 lemma may_be_static_eval_preserved_under_seq_step_down: "
   (\<V>, \<C>) \<Turnstile>\<^sub>\<E> \<E> \<Longrightarrow> leaf \<E> \<pi> \<Longrightarrow> \<E> \<pi> = Some (\<langle>RESULT x; \<rho>; \<langle>x\<^sub>\<kappa>, e\<^sub>\<kappa>, \<rho>\<^sub>\<kappa>\<rangle> # \<kappa>\<rangle>) \<Longrightarrow> 
-  \<langle>RESULT x; \<rho>; \<langle>x\<^sub>\<kappa>, e\<^sub>\<kappa>, \<rho>\<^sub>\<kappa>\<rangle> # \<kappa>\<rangle> \<hookrightarrow> \<sigma>' \<Longrightarrow> (\<V>, \<C>) \<Turnstile>\<^sub>\<E> \<E>(\<pi> ;;(LReturn x\<^sub>\<kappa>) \<mapsto> \<sigma>')
+  \<langle>RESULT x; \<rho>; \<langle>x\<^sub>\<kappa>, e\<^sub>\<kappa>, \<rho>\<^sub>\<kappa>\<rangle> # \<kappa>\<rangle> \<down>\<hookrightarrow> \<sigma>' \<Longrightarrow> (\<V>, \<C>) \<Turnstile>\<^sub>\<E> \<E>(\<pi> ;;(LReturn x\<^sub>\<kappa>) \<mapsto> \<sigma>')
 "
 proof
   
   assume "(\<V>, \<C>) \<Turnstile>\<^sub>\<E> \<E>" and "\<E> \<pi> = Some (\<langle>RESULT x; \<rho>; \<langle>x\<^sub>\<kappa>, e\<^sub>\<kappa>, \<rho>\<^sub>\<kappa>\<rangle> # \<kappa>\<rangle>)" then
   have "(\<V>, \<C>) \<Turnstile>\<^sub>\<sigma> \<langle>RESULT x; \<rho>; \<langle>x\<^sub>\<kappa>, e\<^sub>\<kappa>, \<rho>\<^sub>\<kappa>\<rangle> # \<kappa>\<rangle>" by (simp add: may_be_static_eval_pool.simps)
   
-  assume "\<langle>RESULT x; \<rho>; \<langle>x\<^sub>\<kappa>, e\<^sub>\<kappa>, \<rho>\<^sub>\<kappa>\<rangle> # \<kappa>\<rangle> \<hookrightarrow> \<sigma>'" with `(\<V>, \<C>) \<Turnstile>\<^sub>\<sigma> \<langle>RESULT x; \<rho>; \<langle>x\<^sub>\<kappa>, e\<^sub>\<kappa>, \<rho>\<^sub>\<kappa>\<rangle> # \<kappa>\<rangle>`
-  have "(\<V>, \<C>) \<Turnstile>\<^sub>\<sigma> \<sigma>'" by (simp add: may_be_static_eval_state_preserved_under_step)
+  assume "\<langle>RESULT x; \<rho>; \<langle>x\<^sub>\<kappa>, e\<^sub>\<kappa>, \<rho>\<^sub>\<kappa>\<rangle> # \<kappa>\<rangle> \<down>\<hookrightarrow> \<sigma>'" with `(\<V>, \<C>) \<Turnstile>\<^sub>\<sigma> \<langle>RESULT x; \<rho>; \<langle>x\<^sub>\<kappa>, e\<^sub>\<kappa>, \<rho>\<^sub>\<kappa>\<rangle> # \<kappa>\<rangle>`
+  have "(\<V>, \<C>) \<Turnstile>\<^sub>\<sigma> \<sigma>'" by (simp add: may_be_static_eval_state_preserved_under_step_down)
 
   from \<open>(\<V>, \<C>) \<Turnstile>\<^sub>\<E> \<E>\<close> \<open>(\<V>, \<C>) \<Turnstile>\<^sub>\<sigma> \<sigma>'\<close>
   show "\<forall>\<pi>' \<sigma>. (\<E>(\<pi> ;;(LReturn x\<^sub>\<kappa>) \<mapsto> \<sigma>')) \<pi>' = Some \<sigma> \<longrightarrow> (\<V>, \<C>) \<Turnstile>\<^sub>\<sigma> \<sigma>" by (simp add: may_be_static_eval_pool.simps)
@@ -902,23 +955,23 @@ qed
 
 lemma may_be_static_eval_preserved_under_seq_step_up: "
   (\<V>, \<C>) \<Turnstile>\<^sub>\<E> \<E> \<Longrightarrow> leaf \<E> \<pi> \<Longrightarrow> \<E> \<pi> = Some (\<langle>LET x = b in e; \<rho>; \<kappa>\<rangle>) \<Longrightarrow> 
-  \<langle>LET x = b in e; \<rho>; \<kappa>\<rangle> \<hookrightarrow> \<sigma>' \<Longrightarrow> (\<V>, \<C>) \<Turnstile>\<^sub>\<E> \<E>(\<pi>;;(LCall x) \<mapsto> \<sigma>')
+  \<langle>LET x = b in e; \<rho>; \<kappa>\<rangle> \<up>\<hookrightarrow> \<sigma>' \<Longrightarrow> (\<V>, \<C>) \<Turnstile>\<^sub>\<E> \<E>(\<pi>;;(LCall x) \<mapsto> \<sigma>')
 "
 proof
   assume "(\<V>, \<C>) \<Turnstile>\<^sub>\<E> \<E>" and "\<E> \<pi> = Some (\<langle>LET x = b in e; \<rho>; \<kappa>\<rangle>)" then
   have "(\<V>, \<C>) \<Turnstile>\<^sub>\<sigma> \<langle>LET x = b in e; \<rho>; \<kappa>\<rangle>" by (simp add: may_be_static_eval_pool.simps)
 
-  assume "\<langle>LET x = b in e; \<rho>; \<kappa>\<rangle> \<hookrightarrow> \<sigma>'" with `(\<V>, \<C>) \<Turnstile>\<^sub>\<sigma> \<langle>LET x = b in e; \<rho>; \<kappa>\<rangle>`
-  have "(\<V>, \<C>) \<Turnstile>\<^sub>\<sigma> \<sigma>'" by (simp add: may_be_static_eval_state_preserved_under_step)
+  assume "\<langle>LET x = b in e; \<rho>; \<kappa>\<rangle> \<up>\<hookrightarrow> \<sigma>'" with `(\<V>, \<C>) \<Turnstile>\<^sub>\<sigma> \<langle>LET x = b in e; \<rho>; \<kappa>\<rangle>`
+  have "(\<V>, \<C>) \<Turnstile>\<^sub>\<sigma> \<sigma>'" by (simp add: may_be_static_eval_state_preserved_under_step_up)
 
   from \<open>(\<V>, \<C>) \<Turnstile>\<^sub>\<E> \<E>\<close> \<open>(\<V>, \<C>) \<Turnstile>\<^sub>\<sigma> \<sigma>'\<close>
   show "\<forall>\<pi>' \<sigma>. (\<E>(\<pi> ;;(LCall x) \<mapsto> \<sigma>')) \<pi>' = Some \<sigma> \<longrightarrow> (\<V>, \<C>) \<Turnstile>\<^sub>\<sigma> \<sigma>" by (simp add: may_be_static_eval_pool.simps)
 qed
 
-
+(*
 lemma may_be_static_eval_preserved_under_seq_step: "
   (\<V>, \<C>) \<Turnstile>\<^sub>\<E> \<E> \<Longrightarrow> leaf \<E> \<pi> \<Longrightarrow> \<E> \<pi> = Some (\<langle>LET x = b in e; \<rho>; \<kappa>\<rangle>) \<Longrightarrow> 
-  \<langle>LET x = b in e; \<rho>; \<kappa>\<rangle> \<hookrightarrow> \<sigma>' \<Longrightarrow> (\<V>, \<C>) \<Turnstile>\<^sub>\<E> \<E>(\<pi> ;;(LNext x) \<mapsto> \<sigma>')
+  seq_step (LET x = b in e) \<rho> \<rho>' \<Longrightarrow> (\<V>, \<C>) \<Turnstile>\<^sub>\<E> \<E>(\<pi> ;;(LNext x) \<mapsto> \<langle>e; \<rho>'; \<kappa>\<rangle>)
 "
 proof
   assume "(\<V>, \<C>) \<Turnstile>\<^sub>\<E> \<E>" and "\<E> \<pi> = Some (\<langle>LET x = b in e; \<rho>; \<kappa>\<rangle>)" then
@@ -930,6 +983,7 @@ proof
   from \<open>(\<V>, \<C>) \<Turnstile>\<^sub>\<E> \<E>\<close> \<open>(\<V>, \<C>) \<Turnstile>\<^sub>\<sigma> \<sigma>'\<close>
   show "\<forall>\<pi>' \<sigma>. (\<E>(\<pi> ;;(LNext x) \<mapsto> \<sigma>')) \<pi>' = Some \<sigma> \<longrightarrow> (\<V>, \<C>) \<Turnstile>\<^sub>\<sigma> \<sigma>" by (simp add: may_be_static_eval_pool.simps)
 qed
+*)
 
 lemma may_be_static_eval_pool_to_exp_let: "
   (\<V>, \<C>) \<Turnstile>\<^sub>\<E> \<E> \<Longrightarrow>
@@ -1362,32 +1416,43 @@ theorem may_be_static_eval_preserved_under_concur_step : "
   (\<V>, \<C>) \<Turnstile>\<^sub>\<E> \<E>'
 "
 proof -
-  assume "(\<V>, \<C>) \<Turnstile>\<^sub>\<E> \<E>"
-  assume "\<E> \<rightarrow> \<E>'" then
-  show "(\<V>, \<C>) \<Turnstile>\<^sub>\<E> \<E>'"
+  assume 
+    H1: "(\<V>, \<C>) \<Turnstile>\<^sub>\<E> \<E>" and
+    H2: "\<E> \<rightarrow> \<E>'"
+
+  from H2 show "(\<V>, \<C>) \<Turnstile>\<^sub>\<E> \<E>'"
   proof cases
     case (Seq_Step_Down \<pi> x \<rho> x\<^sub>\<kappa> e\<^sub>\<kappa> \<rho>\<^sub>\<kappa> \<kappa> \<sigma>')
-    assume "\<E>' = \<E> ++ [\<pi> ;; (LReturn x\<^sub>\<kappa>) \<mapsto> \<sigma>']"
-    assume "leaf \<E> \<pi>" and "\<E> \<pi> = Some (\<langle>RESULT x;\<rho>;\<langle>x\<^sub>\<kappa>,e\<^sub>\<kappa>,\<rho>\<^sub>\<kappa>\<rangle> # \<kappa>\<rangle>)"
-    and "\<langle>RESULT x;\<rho>;\<langle>x\<^sub>\<kappa>,e\<^sub>\<kappa>,\<rho>\<^sub>\<kappa>\<rangle> # \<kappa>\<rangle> \<hookrightarrow> \<sigma>'"
-    with \<open>(\<V>, \<C>) \<Turnstile>\<^sub>\<E> \<E>\<close>
-    have "(\<V>, \<C>) \<Turnstile>\<^sub>\<E> \<E>(\<pi> ;; (LReturn x\<^sub>\<kappa>) \<mapsto> \<sigma>')" by (simp add:  may_be_static_eval_preserved_under_seq_step_down)
-    with `\<E>' = \<E> ++ [\<pi> ;; (LReturn x\<^sub>\<kappa>) \<mapsto> \<sigma>']`
-    show "(\<V>, \<C>) \<Turnstile>\<^sub>\<E> \<E>'" by simp
+
+    assume 
+      H3: "\<E>' = \<E> ++ [\<pi> ;; (LReturn x\<^sub>\<kappa>) \<mapsto> \<sigma>']" and
+      H4: "leaf \<E> \<pi>" and 
+      H5: "\<E> \<pi> = Some (\<langle>RESULT x;\<rho>;\<langle>x\<^sub>\<kappa>,e\<^sub>\<kappa>,\<rho>\<^sub>\<kappa>\<rangle> # \<kappa>\<rangle>)" and 
+      H6: "\<langle>RESULT x;\<rho>;\<langle>x\<^sub>\<kappa>,e\<^sub>\<kappa>,\<rho>\<^sub>\<kappa>\<rangle> # \<kappa>\<rangle> \<down>\<hookrightarrow> \<sigma>'"
+
+    with H1 have "(\<V>, \<C>) \<Turnstile>\<^sub>\<E> \<E>(\<pi> ;; (LReturn x\<^sub>\<kappa>) \<mapsto> \<sigma>')" by (simp add:  may_be_static_eval_preserved_under_seq_step_down)
+    
+    with H3 show "(\<V>, \<C>) \<Turnstile>\<^sub>\<E> \<E>'" by simp
   next
-    case (Seq_Step \<pi> x b e \<rho> \<kappa> \<rho>')
-    assume "\<E>' = \<E> ++ [\<pi> ;; (LNext x) \<mapsto> \<langle>e;\<rho>';\<kappa>\<rangle>]"
-    assume "leaf \<E> \<pi>" and "\<E> \<pi> = Some (\<langle>LET x = b in e;\<rho>;\<kappa>\<rangle>)"
-    and "\<langle>LET x = b in e;\<rho>;\<kappa>\<rangle> \<hookrightarrow> \<langle>e;\<rho>';\<kappa>\<rangle>"
-    with \<open>(\<V>, \<C>) \<Turnstile>\<^sub>\<E> \<E>\<close>
-    have "(\<V>, \<C>) \<Turnstile>\<^sub>\<E> \<E>(\<pi> ;; (LNext x) \<mapsto> \<langle>e;\<rho>';\<kappa>\<rangle>)" by (simp add: may_be_static_eval_preserved_under_seq_step)
-    with \<open>\<E>' = \<E> ++ [\<pi> ;; (LNext x) \<mapsto> \<langle>e;\<rho>';\<kappa>\<rangle>]\<close>
-    show "(\<V>, \<C>) \<Turnstile>\<^sub>\<E> \<E>'" by simp
+    case (Seq_Step \<pi> x b e \<rho> \<kappa> \<omega>)
+    assume 
+      H3: "\<E>' = \<E> ++ [\<pi> ;; (LNext x) \<mapsto> \<langle>e;\<rho>(x \<mapsto> \<omega>);\<kappa>\<rangle>]" and
+      H4: "leaf \<E> \<pi>" and 
+      H5: "\<E> \<pi> = Some (\<langle>LET x = b in e;\<rho>;\<kappa>\<rangle>)" and 
+      H6: "seq_step (b, \<rho>) \<omega>"
+
+    from H1 H5 have H7:"(\<V>, \<C>) \<Turnstile>\<^sub>\<sigma> \<langle>LET x = b in e;\<rho>;\<kappa>\<rangle>" by (auto simp: may_be_static_eval_pool.simps)
+
+    with H6 have H8: "(\<V>, \<C>) \<Turnstile>\<^sub>\<sigma> \<langle>e;\<rho>(x \<mapsto> \<omega>);\<kappa>\<rangle>" by (auto simp: may_be_static_eval_state_preserved_under_step)
+
+    with H1 have "(\<V>, \<C>) \<Turnstile>\<^sub>\<E> \<E>(\<pi> ;; (LNext x) \<mapsto> \<langle>e;\<rho>(x \<mapsto> \<omega>);\<kappa>\<rangle>)" by (auto simp: may_be_static_eval_pool.simps)
+
+    with H3 show "(\<V>, \<C>) \<Turnstile>\<^sub>\<E> \<E>'" by simp
   next
     case (Seq_Step_Up \<pi> x b e \<rho> \<kappa> e' \<rho>')
     assume "\<E>' = \<E> ++ [\<pi> ;; (LCall x) \<mapsto> \<langle>e';\<rho>';\<langle>x,e,\<rho>\<rangle> # \<kappa>\<rangle>]"
     assume "leaf \<E> \<pi>" and "\<E> \<pi> = Some (\<langle>LET x = b in e;\<rho>;\<kappa>\<rangle>)"
-    and "\<langle>LET x = b in e;\<rho>;\<kappa>\<rangle> \<hookrightarrow> \<langle>e';\<rho>';\<langle>x,e,\<rho>\<rangle> # \<kappa>\<rangle>"
+    and "\<langle>LET x = b in e;\<rho>;\<kappa>\<rangle> \<up>\<hookrightarrow> \<langle>e';\<rho>';\<langle>x,e,\<rho>\<rangle> # \<kappa>\<rangle>"
     with \<open>(\<V>, \<C>) \<Turnstile>\<^sub>\<E> \<E>\<close>
     have "(\<V>, \<C>) \<Turnstile>\<^sub>\<E> \<E>(\<pi> ;; (LCall) x \<mapsto> \<langle>e';\<rho>';\<langle>x,e,\<rho>\<rangle> # \<kappa>\<rangle>)" by (simp add: may_be_static_eval_preserved_under_seq_step_up)
     with \<open>\<E>' = \<E> ++ [\<pi> ;; (LCall x) \<mapsto> \<langle>e';\<rho>';\<langle>x,e,\<rho>\<rangle> # \<kappa>\<rangle>]\<close>
